feat(TM): rework transition function (WIP)
problem: the intended TM encoding should be injective.
this is not actually possible with the current definition; as the types of states and symbols can be infinite, the range of the transition function(s) can be as well.
this is not interesting/useful for reasoning about TMs and causes TMs to have an infinite amount of "variants" that all have the same encoding, but are not "equal" as far as Isabelle's `HOL.eq` (equivalent to `Pure.eq` in HOL) is concerned.

proposed solution: add axioms to valid_TM that fix/define the behavior of the transition function (next_state, next_write, next_move) in the "undefined" range (for non-well-formed/invalid input values).
for two TMs to be equal (`HOL.eq`) it then suffices for their transition functions to have equal results in the intended range.

Note: this approach works due to function extensionability (`thm HOL.ext`)

TM.thy
@@ -146,7 +146,7 @@ text\<open>To use TMs conveniently, we setup a type and a locale as follows:
 
   A simpler form of this pattern has been used to define the type of filters (\<^typ>\<open>'a filter\<close>).\<close>
 
-locale valid_TM =
+locale valid_TM_not_uniq =
   fixes M :: "('q, 's) TM_record"
   assumes at_least_one_tape: "tape_count M > 0" (* TODO motivate this assm. "why is this necessary?" edit: initial_config would have to be defined differently *)
     and symbol_axioms: "finite (symbols M)" "symbols M \<noteq> {}"
@@ -155,24 +155,136 @@ locale valid_TM =
     and next_state_valid: "\<And>q hds. q \<in> states M \<Longrightarrow> wf_hds_rec M hds \<Longrightarrow> next_state M q hds \<in> states M"
     and next_write_valid: "\<And>q hds i. q \<in> states M \<Longrightarrow> wf_hds_rec M hds \<Longrightarrow> i < tape_count M \<Longrightarrow>
           next_write M q hds i \<in> tape_symbols_rec M"
+begin
+lemmas axioms = at_least_one_tape symbol_axioms state_axioms next_state_valid next_write_valid
+end
+
+locale valid_TM = valid_TM_not_uniq +
+  \<comment> \<open>Require canonical default values for the transition function outside its intended definition range.
+      There are two simple options for choosing default values:
+
+      \<^bold>\<open>Canonical values\<close>. Use values that are always available in the context of TMs.
+      This would result in the initial state \<open>q\<^sub>0\<close>, the \<open>blank_symbol\<close> and \<open>No_Shift\<close>.
+
+      \<^bold>\<open>No-Op\<close>. Simply output the respective input value.
+      Semantically, this relates to the TM looping endlessly in a constant configuration.
+      This approach is somewhat problematic for \<open>next_write\<close>, as \<open>hds ! i\<close> is not defined for all values.
+      This means that all functions will have to be defined with exactly \<open>hds ! i\<close> for out-of-bounds inputs,
+      as it is the only value for which equality can be shown in Isabelle.
+
+      We choose the second approach as we suspect it will integrate better with simple definitions.\<close>
+  assumes next_state_default: "\<And>q hds. q \<notin> states M \<Longrightarrow> next_state M q hds = q"
+    "\<And>q hds. \<not> wf_hds_rec M hds \<Longrightarrow> next_state M q hds = q"
+    and next_write_default:   "\<And>q hds i. q \<notin> states M \<Longrightarrow> next_write M q hds i = hds ! i" (* TODO evaluate if this works out. should make things a bit easier, but could lead to unprovable goals *)
+    "\<And>q hds i. \<not> wf_hds_rec M hds \<Longrightarrow> next_write M q hds i = hds ! i"
+    "\<And>q hds i. \<not> i < tape_count M \<Longrightarrow> next_write M q hds i = hds ! i"
+    and next_move_default:    "\<And>q hds i. q \<notin> states M \<Longrightarrow> next_move M q hds i = No_Shift"
+    "\<And>q hds i. \<not> wf_hds_rec M hds \<Longrightarrow> next_move M q hds i = No_Shift"
+    "\<And>q hds i. \<not> i < tape_count M \<Longrightarrow> next_move M q hds i = No_Shift"
+
+
+lemma "wf_hds_rec M hds \<Longrightarrow> i < tape_count M \<Longrightarrow> hds ! i \<in> tape_symbols_rec M" by force
+
+definition next_fun_wrapper :: "['x, nat, 's set, 'q set, 'q \<Rightarrow> 's option list \<Rightarrow> nat \<Rightarrow> 'x, 'q, 's option list, nat] \<Rightarrow> 'x"
+  where "next_fun_wrapper default_val k \<Sigma> Q f q hds i \<equiv> if q \<in> Q \<and> length hds = k \<and> set hds \<subseteq> options \<Sigma> \<and> i < k then f q hds i else default_val"
+
+abbreviation next_state_wrapper :: "[nat, 's set, 'q set, 'q \<Rightarrow> 's option list \<Rightarrow> 'q, 'q, 's option list] \<Rightarrow> 'q"
+  where "next_state_wrapper k \<Sigma> Q f q hds \<equiv> next_fun_wrapper q k \<Sigma> Q (\<lambda>q hds i. f q hds) q hds 0"
+abbreviation next_write_wrapper :: "[nat, 's set, 'q set, 'q \<Rightarrow> 's option list \<Rightarrow> nat \<Rightarrow> 's option, 'q, 's option list, nat] \<Rightarrow> 's option"
+  where "next_write_wrapper k \<Sigma> Q f q hds i \<equiv> next_fun_wrapper (hds ! i) k \<Sigma> Q f q hds i"
+abbreviation next_move_wrapper :: "[nat, 's set, 'q set, 'q \<Rightarrow> 's option list \<Rightarrow> nat \<Rightarrow> head_move, 'q, 's option list, nat] \<Rightarrow> head_move"
+  where "next_move_wrapper k \<Sigma> Q f q hds i \<equiv> next_fun_wrapper No_Shift k \<Sigma> Q f q hds i"
+
+lemma next_fun_wrapper_default[simp]:
+  fixes k \<Sigma> Q f val and M :: "('q, 's) TM_record"
+  defines "f' \<equiv> next_fun_wrapper val k \<Sigma> Q f"
+  defines "f'' \<equiv> next_fun_wrapper val (tape_count M) (symbols M) (states M) f"
+  shows "q \<notin> Q \<Longrightarrow> f' q hds i = val"
+    and "length hds \<noteq> k \<Longrightarrow> f' q hds i = val"
+    and "\<not> set hds \<subseteq> options \<Sigma> \<Longrightarrow> f' q hds i = val"
+    and "\<not> i < k \<Longrightarrow> f' q hds i = val"
+    and "\<not> wf_hds_rec M hds \<Longrightarrow> f'' q hds i = val"
+  unfolding assms next_fun_wrapper_def by (blast intro!: if_not_P)+
+
+lemma next_fun_wrapper_simps[simp]:
+  fixes k \<Sigma> Q f val and M :: "('q, 's) TM_record"
+  defines "f' \<equiv> next_fun_wrapper val k \<Sigma> Q f"
+  defines "f'' \<equiv> next_fun_wrapper val (tape_count M) (symbols M) (states M) f"
+  shows "q \<in> Q \<Longrightarrow> length hds = k \<Longrightarrow> set hds \<subseteq> options \<Sigma> \<Longrightarrow> i < k \<Longrightarrow> f' q hds i = f q hds i"
+    and "q \<in> states M \<Longrightarrow> wf_hds_rec M hds \<Longrightarrow> i < tape_count M \<Longrightarrow> f'' q hds i = f q hds i"
+  unfolding assms next_fun_wrapper_def using assms(2-) by (blast intro!: if_P)+
+
+lemma next_state_wrapper_simps[simp]:
+  fixes k \<Sigma> Q f val
+  defines "f' \<equiv> next_fun_wrapper val k \<Sigma> Q f"
+  assumes "q \<in> Q" and "length hds = k" and "set hds \<subseteq> options \<Sigma>"
+  shows "k > 0 =simp=> f' q hds 0 = f q hds 0"
+  using assms unfolding f'_def by (intro simp_impliesI, subst next_fun_wrapper_simps) fastforce+
+
+
+definition TM_default_wrapper :: "('q, 's) TM_record \<Rightarrow> ('q, 's) TM_record"
+  where "TM_default_wrapper M \<equiv> M\<lparr>
+    next_state := next_state_wrapper (tape_count M) (symbols M) (states M) (next_state M),
+    next_write := next_write_wrapper (tape_count M) (symbols M) (states M) (next_write M),
+    next_move := next_move_wrapper (tape_count M) (symbols M) (states M) (next_move M)
+  \<rparr>"
+
+lemma TM_default_wrapper_simps[simp]:
+  fixes M :: "('q, 's) TM_record"
+  defines "M' \<equiv> TM_default_wrapper M"
+  shows "tape_count M' = tape_count M"
+    and "symbols M' = symbols M"
+    and "states M' = states M"
+    and "initial_state M' = initial_state M"
+    and "final_states M' = final_states M"
+    and "accepting_states M' = accepting_states M"
+    and "next_state M' = next_state_wrapper (tape_count M) (symbols M) (states M) (next_state M)"
+    and "next_write M' = next_write_wrapper (tape_count M) (symbols M) (states M) (next_write M)"
+    and "next_move M' = next_move_wrapper (tape_count M) (symbols M) (states M) (next_move M)"
+    and "wf_hds_rec M' = wf_hds_rec M"
+  unfolding M'_def TM_default_wrapper_def by (induction M) force+
 
 text\<open>Notes on assumptions.
   Many of these assumptions would be trivial to satisfy when explicitly constructing a TM,
   especially the premises of \<open>next_state_valid\<close> and \<open>next_write_valid\<close>.
   They are, however, very useful when constructing TMs from other TMs.\<close>
 
-lemma valid_TM_I:
+
+lemma valid_TM_wrapper[simp]: "valid_TM (TM_default_wrapper M) \<longleftrightarrow> valid_TM_not_uniq M"
+  (is "valid_TM ?M' \<longleftrightarrow> _")
+proof -
+  note * = TM_default_wrapper_simps next_fun_wrapper_simps
+  have h1: "valid_TM_axioms ?M'"
+    using next_fun_wrapper_default
+    by (unfold_locales, unfold *)
+  have h2: "valid_TM_not_uniq ?M'" if "valid_TM_not_uniq M"
+    using valid_TM_not_uniq.axioms[OF that]
+    by (unfold_locales, unfold *)
+
+  show ?thesis
+  proof (rule iffI)
+    from h1 h2 show "valid_TM_not_uniq M \<Longrightarrow> valid_TM ?M'" by (intro_locales) blast+
+
+    assume "valid_TM ?M'"
+    then have "valid_TM_not_uniq ?M'" by (fact valid_TM.axioms)
+    note valid_TM_not_uniq.axioms[OF this, simplified]
+    then show "valid_TM_not_uniq M" by (unfold_locales) (unfold next_fun_wrapper_simps)
+  qed
+qed
+
+lemma valid_TM_I[intro]:
   fixes k \<Sigma> Q q\<^sub>0 F F\<^sub>A \<delta>\<^sub>q \<delta>\<^sub>w \<delta>\<^sub>m
-  defines "(M :: ('q, 's) TM_record) \<equiv> \<lparr> TM_record.tape_count = k, symbols = \<Sigma>,
+  defines "(M :: ('q, 's) TM_record) \<equiv>  \<lparr> TM_record.tape_count = k, symbols = \<Sigma>,
     states = Q, initial_state = q\<^sub>0, final_states = F, accepting_states = F\<^sub>A,
     next_state = \<delta>\<^sub>q, next_write = \<delta>\<^sub>w, next_move = \<delta>\<^sub>m \<rparr>"
-  defines "\<Sigma>\<^sub>t\<^sub>p \<equiv> options \<Sigma>"
+  defines [simp]: "\<Sigma>\<^sub>t\<^sub>p \<equiv> options \<Sigma>"
   assumes at_least_one_tape: "k > 0"
     and symbol_axioms: "finite \<Sigma>" "\<Sigma> \<noteq> {}"
     and state_axioms: "finite Q" "q\<^sub>0 \<in> Q" "F \<subseteq> Q" "F\<^sub>A \<subseteq> F"
     and next_state_valid: "\<And>q hds. q \<in> Q \<Longrightarrow> length hds = k \<Longrightarrow> set hds \<subseteq> \<Sigma>\<^sub>t\<^sub>p \<Longrightarrow> \<delta>\<^sub>q q hds \<in> Q"
     and next_write_valid: "\<And>q hds i. q \<in> Q \<Longrightarrow> length hds = k \<Longrightarrow> set hds \<subseteq> \<Sigma>\<^sub>t\<^sub>p \<Longrightarrow> i < k \<Longrightarrow> \<delta>\<^sub>w q hds i \<in> \<Sigma>\<^sub>t\<^sub>p"
-  shows "valid_TM M"
+  shows "valid_TM (TM_default_wrapper M)"
+  unfolding valid_TM_wrapper
 proof (unfold_locales, unfold M_def TM_record.simps wf_hds_rec_simps)
   fix q hds
   assume "q \<in> Q" and wf: "length hds = k \<and> set hds \<subseteq> options \<Sigma>"
@@ -187,9 +299,10 @@ lemma valid_TM_finiteI:
   assumes at_least_one_tape: "tape_count M > 0"
     and symbols_UNIV: "symbols M = UNIV"
     and state_axioms: "finite (states M)" "initial_state M \<in> states M"
-      "final_states M \<subseteq> states M" "accepting_states M \<subseteq> final_states M"
+    "final_states M \<subseteq> states M" "accepting_states M \<subseteq> final_states M"
     and next_state_valid: "\<And>q hds. q \<in> states M \<Longrightarrow> next_state M q hds \<in> states M"
-  shows "valid_TM M"
+  shows "valid_TM (TM_default_wrapper M)"
+  unfolding valid_TM_wrapper
 proof
   show "finite (symbols M)" by (fact finite_class.finite)
   show "symbols M \<noteq> {}" unfolding symbols_UNIV by (fact UNIV_not_empty)
@@ -200,7 +313,7 @@ proof
   show "next_write M q hds i \<in> tape_symbols_rec M" unfolding symbols_UNIV by simp
 qed (fact assms)+
 
-lemma valid_TM_finiteI':
+lemma valid_TM_finiteI'[intro]:
   fixes k Q q\<^sub>0 F F\<^sub>A \<delta>\<^sub>q \<delta>\<^sub>w \<delta>\<^sub>m
   defines "(M :: ('q, 's::finite) TM_record) \<equiv> \<lparr> TM_record.tape_count = k, symbols = UNIV,
     states = Q, initial_state = q\<^sub>0, final_states = F, accepting_states = F\<^sub>A,
@@ -208,7 +321,7 @@ lemma valid_TM_finiteI':
   assumes at_least_one_tape: "k > 0"
     and state_axioms: "finite Q" "q\<^sub>0 \<in> Q" "F \<subseteq> Q" "F\<^sub>A \<subseteq> F"
     and next_state_valid: "\<And>q hds. q \<in> Q \<Longrightarrow> \<delta>\<^sub>q q hds \<in> Q"
-  shows "valid_TM M"
+  shows "valid_TM (TM_default_wrapper M)"
 proof (intro valid_TM_finiteI, unfold M_def TM_record.simps)
   show "UNIV = UNIV" ..
 qed (fact assms)+
@@ -218,14 +331,14 @@ text\<open>To define a type, we must prove that it is inhabited (there exist ele
   For this we define the trivial ``rejecting TM'', and prove it to be valid.\<close>
 
 definition rejecting_TM_rec :: "'q \<Rightarrow> 's \<Rightarrow> ('q, 's) TM_record"
-  where "rejecting_TM_rec q0 s \<equiv> \<lparr>
+  where "rejecting_TM_rec q0 s \<equiv> TM_default_wrapper \<lparr>
   tape_count = 1, symbols = {s},
   states = {q0}, initial_state = q0, final_states = {q0}, accepting_states = {},
   next_state = (\<lambda>q hds. q0), next_write = (\<lambda>q hds i. blank_symbol), next_move = (\<lambda>q hds i. No_Shift)
 \<rparr>"
 
 lemma rejecting_TM_valid: "valid_TM (rejecting_TM_rec q0 s)"
-  by (unfold_locales, unfold rejecting_TM_rec_def TM_record.simps) blast+
+  unfolding rejecting_TM_rec_def by blast
 
 text\<open>The type \<open>TM\<close> is then defined as the set of valid \<open>TM_record\<close>s.\<close>
 (* TODO elaborate on the implications of this *)
@@ -603,6 +716,21 @@ proof -
 qed
 
 lemma wf_config_last[dest, intro]: "wf_config c \<Longrightarrow> set_tape (last (tapes c)) \<subseteq> \<Sigma>" by auto
+
+lemma next_fun_wrapper_simps[simplified, simp]:
+  fixes f val c
+  defines "q \<equiv> state c"
+    and "hds \<equiv> heads c"
+    and "f' \<equiv> next_fun_wrapper val k \<Sigma> Q f"
+  assumes "wf_config c"
+  shows "i < k \<Longrightarrow> f' q hds i = f q hds i"
+    and "f' q hds 0 = f q hds 0"
+proof -
+  from \<open>wf_config c\<close> show "i < k \<Longrightarrow> f' q hds i = f q hds i" for i
+    unfolding assms by (subst next_fun_wrapper_simps) blast+
+  then show "f' q hds 0 = f q hds 0" by blast
+qed
+
 
 end \<comment> \<open>\<^locale>\<open>TM\<close>\<close>
 
